\chapter{Intuition}\label{appendix:intuitions}

\section{Tariff}\label{appendix:intuitions_tariff}

First, we express $P_F$ as a function of $t$ and the elasticities.

Starting from the equation 
$$
D_H - S_H = S_F - D_F,
$$ 
and using the definitions of demand and supply, we obtain:
$$
D_H^0\left(1+\epsilon_H \frac{P_H - P_H^0}{P_H^0}\right) - S_H^0\left(1+\eta_H \frac{P_H - P_H^0}{P_H^0}\right) = S_F^0 \left(1+\eta_F \frac{P_F - P_F^0}{P_F^0}\right) - D_F^0\left(1+\epsilon_F \frac{P_F - P_F^0}{P_F^0}\right).
$$
We then factorize by $\frac{P_i-P_i^0}{P_i^0}$ for $i = H,F$:
$$
\frac{P_H - P_H^0}{P_H^0} [D_H^0 \epsilon_H - S_H^0 \eta_H] + D_H^0 - S_H^0 = \frac{P_F - P_F^0}{P_F^0} [S_F^0 \eta_F - D_F^0 \epsilon_F] + S_F^0 - D_F^0.
$$
Noting that $D_H^0 - S_H^0 = S_F^0 - D_F^0$, we obtain:
$$
\frac{P_H - P_H^0}{P_H^0} [D_H^0 \epsilon_H - S_H^0 \eta_H] = \frac{P_F - P_F^0}{P_F^0} [S_F^0 \eta_F - D_F^0 \epsilon_F].
$$

Using the aggregated elasticities defined in Chapter \ref{Sec_tariff}, we have 
$$
\frac{P_F}{P_F^0}= -\frac{\mu_H (1 - t/P_H^0) - \chi_F}{\eta-\epsilon}\frac{X_F^0}{D^0}.
$$

Multiplying both sides by $P_F^0$, a straightforward derivation yields:
$$
\frac{\partial P_F}{\partial t} = \frac{\mu_H}{\eta - \epsilon} \frac{X_F^0}{D^0} \frac{P_F^0}{P_H^0} < 0.
$$

Assuming an initial tariff of zero, i.e. $P_F^0 = P_H^0$, we have:
$$
\frac{P_F}{P_F^0} = - \frac{(1 - t/P_H^0)\mu_H - \chi_F}{\chi_F - \mu_H} = 1+\frac{\mu_H}{\chi_F - \mu_H}\frac{t}{P_H^0}.
$$

Assuming an initial tariff of zero and uniform elasticities across countries, the price and its derivative are given by:
\begin{align*}
P_F &= P_F^0 + t \frac{\mu_H}{\eta_i - \epsilon_i} \frac{X_F^0}{D^0}, \\
\frac{\partial P_F}{\partial t} &= \frac{\mu_H}{\eta_i - \epsilon_i} \frac{X_F^0}{D^0} < 0.
\end{align*}

Regarding total production $Q$, with an initial tariff of zero we have:
\begin{align*}
Q &= Q^0 + \frac{- \frac{t}{P_H^0}\eta_i(S_H^0 \chi_F + S_F^0 \mu_H)}{\mu_H - \chi_F}, \\
\frac{\partial Q}{\partial t} &= \eta_i \frac{S_H^0 \chi_F + S_F^0 \mu_H}{\chi_F - \mu_H}\frac{1}{P_H^0}.
\end{align*}

For emissions, using $E_i = e_i S_i$, we obtain the results presented in Section \ref{Sec_tariff}. In addition, assuming an initial tariff of zero and equal elasticities (i.e., $\eta_H = \eta_F = \eta_i$ and $\epsilon_H = \epsilon_F = \epsilon_i$), we have:
\begin{align*}
E &= E^0 + \frac{\frac{t}{P_H^0} \eta_i (E_H^0 \chi_F + E_F^0 \mu_H)}{\chi_F - \mu_H}, \\[1mm]
\frac{\partial E}{\partial t} &= \eta_i \frac{E_H^0 \chi_F + E_F^0 \mu_H}{\chi_F - \mu_H}\frac{1}{P_H^0}.
\end{align*}

\section{Subvention}\label{appendix:intuitions_subvention}

By rewriting the equilibrium equation with the new supply functions,
$$
D_H^0\left(1+\epsilon_H \frac{P - P^0}{P^0}\right) - S_H^0\left(1+\eta_H \frac{P + s - P^0}{P^0}\right) = S_F^0 \left(1+\eta_F \frac{P - P^0}{P^0}\right) - D_F^0\left(1+\epsilon_F \frac{P - P^0}{P^0}\right),
$$
we obtain the price and its derivative as presented in Section \ref{Sec_subvention}.

When elasticities are uniform across countries, so that $\epsilon_i = \epsilon$ and $\eta_i = \eta$, we have:
\begin{align*}
\frac{P}{P^0} &= 1 + \frac{\eta}{\mu_H - \chi_F} \frac{s S_H^0}{P^0 X_F^0}, \\
\frac{\partial P}{\partial s} &= -\frac{\eta}{\chi_F - \mu_H} \frac{S_H^0}{X_F^0} < 0.
\end{align*}

With regard to supply, we have:
$$
S = S_F + S_H =  S^0 + S^0 \eta \frac{P- P^0}{P^0} + S_H \eta_H \frac{s}{P^0},
$$
which yields the results in Section \ref{Sec_subvention}.

For emissions, using again $E = e_H S_H + e_F S_F$, in the case of uniform elasticities the introduction of the subsidy results in higher emissions only if
$$
\frac{E_H^0}{\eta S_H^0} > \frac{E^0}{(\eta - \epsilon)S^0}.
$$
